theories/rust_typing/shr_ref.v
@@ -1162,9 +1162,10 @@ Section rules.
   Global Instance stratify_ltype_shared_inst1 {rt} π E L mu mdu {M} (ml : M) l (lt : ltype rt) κ (r : place_rfn rt) :
     StratifyLtype π E L mu mdu StratRefoldFull ml l lt r (Shared κ) | 100 :=
     λ T, i2p (stratify_ltype_shared π E L mu mdu StratRefoldFull ml l lt κ r T).
-  Global Instance stratify_ltype_shared_inst2 {rt} π E L mu mdu {M} (ml : M) l (lt : ltype rt) κ (r : place_rfn rt) :
-    StratifyLtype π E L mu mdu StratRefoldOpened ml l lt r (Shared κ) | 100 :=
-    λ T, i2p (stratify_ltype_shared π E L mu mdu StratRefoldOpened ml l lt κ r T).
+  (* TODO needed? *)
+  (*Global Instance stratify_ltype_shared_inst2 {rt} π E L mu mdu {M} (ml : M) l (lt : ltype rt) κ (r : place_rfn rt) :*)
+    (*StratifyLtype π E L mu mdu StratRefoldOpened ml l lt r (Shared κ) | 100 :=*)
+    (*λ T, i2p (stratify_ltype_shared π E L mu mdu StratRefoldOpened ml l lt κ r T).*)
 
   Lemma stratify_ltype_ofty_shr {rt} π E L mu ma {M} (ml : M) l (ty : type rt) κ (r : place_rfn (place_rfn rt)) b T :
     stratify_ltype π E L mu StratDoUnfold ma ml l (ShrLtype (◁ ty) κ) r b T
